spec-checker-ocaml/fstar-compiler/specs/poly1305.fst
@@ -1,0 +1,49 @@
+(* Generated from hacspec module ../specs/poly1305.py *)
+module Poly1305
+open Speclib
+let blocksize: int = 16
+let block_t: Type0 = array_t uint8_t 16
+let key_t: Type0 = array_t uint8_t 32
+let tag_t: Type0 = array_t uint8_t 16
+let subblock_t: Type0 = (x: vlarray_t uint8_t {(bytes_length x) <=. 16})
+let p130m5: nat = (2 **. 130) -. 5
+let felem_t: Type0 = natmod_t p130m5
+let felem (n: nat) : natmod_t p130m5 = natmod n p130m5
+let encode (block: (x: vlarray_t uint8_t {(bytes_length x) <=. 16})) : natmod_t p130m5 =
+  let b = array_create 16 (uint8 0) in
+  let b = array_update_slice b 0 (bytes_length block) block in
+  let welem = felem (bytes_to_nat_le b) in
+  let lelem = felem (2 **. (8 *. (array_length block))) in
+  lelem +. welem
+let encode_r (r: array_t uint8_t 16) : natmod_t p130m5 =
+  let ruint = bytes_to_uint128_le r in
+  let ruint = ruint &. (uint128 21267647620597763993911028882763415551) in
+  let r_nat = uintn_to_nat ruint in
+  felem r_nat
+let poly (text: vlarray_t uint8_t) (r: natmod_t p130m5) : natmod_t p130m5 =
+  let blocks, last = array_split_blocks text blocksize in
+  let acc = felem 0 in
+  let acc =
+    repeati (array_length blocks)
+      (fun i acc ->
+          let acc = (acc +. (encode blocks.[ i ])) *. r in
+          acc)
+      acc
+  in
+  let acc =
+    if (array_length last) >. 0
+    then
+      (let acc = (acc +. (encode last)) *. r in
+        acc)
+    else acc
+  in
+  acc
+let poly1305_mac (text: vlarray_t uint8_t) (k: array_t uint8_t 32) : array_t uint8_t 16 =
+  let r = array_slice k 0 blocksize in
+  let s = array_slice k blocksize (2 *. blocksize) in
+  let relem = encode_r r in
+  let selem = bytes_to_uint128_le s in
+  let a = poly text relem in
+  let n = (uint128 ((natmod_to_nat a) % (2 **. 128))) +. selem in
+  bytes_from_uint128_le n
+
